theories/L6_PCPS/closure_conversion_invariants.v
@@ -71,7 +71,7 @@ Section Closure_conversion_invariants.
                       ~ In _ Funs x ->
                       ~ In _ GFuns x ->
                       M.get x rho = Some v ->
-                      cc_approx_val cenv clo_tag k boundG v v') FVs vs.
+                      cc_approx_val clo_tag k boundG v v') FVs vs.
   
   (** Invariant about the free variables *) 
   Definition FV_inv k rho rho' Scope Funs GFuns c Γ FVs : Prop :=
@@ -84,7 +84,7 @@ Section Closure_conversion_invariants.
                       ~ In _ Funs x ->
                       ~ In _ GFuns x ->
                       M.get x rho = Some v ->
-                      cc_approx_val cenv clo_tag k boundG v v') FVs vs.
+                      cc_approx_val clo_tag k boundG v v') FVs vs.
   
   (** Invariant about the free variables *) 
   Definition FV_inv_strong k rho rho' Scope Funs GFuns c Γ FVs : Prop :=
@@ -96,7 +96,7 @@ Section Closure_conversion_invariants.
                       ~ In _ Funs x ->
                       ~ In _ GFuns x ->
                       M.get x rho = Some v ->
-                      cc_approx_val cenv clo_tag k boundG v v') FVs vs.
+                      cc_approx_val clo_tag k boundG v v') FVs vs.
 
   
   (** Invariant about the functions in the current function definition *)
@@ -110,7 +110,7 @@ Section Closure_conversion_invariants.
         v = (Vfun rho1 B1 f1) /\
         ~ In _ Scope f /\
         M.get f rho' = Some (Vfun rho2 B2 f2) /\
-        cc_approx_val cenv clo_tag k boundG
+        cc_approx_val clo_tag k boundG
                       (Vfun rho1 B1 f1)
                       (Vconstr clo_tag [(Vfun rho2 B2 f2) ; env]).
 
@@ -123,7 +123,7 @@ Section Closure_conversion_invariants.
       exists rho1 B1 f1 rho2 B2 f2,
         v = (Vfun rho1 B1 f1) /\
         M.get f rho' = Some (Vfun rho2 B2 f2) /\
-        cc_approx_val cenv clo_tag k boundG
+        cc_approx_val clo_tag k boundG
                       (Vfun rho1 B1 f1)
                       (Vconstr clo_tag [(Vfun rho2 B2 f2) ; (Vconstr c [])]).
 
@@ -153,7 +153,7 @@ Section Closure_conversion_invariants.
 
     
     M.get (genv f) rho' = Some env ->
-    (cc_approx_val cenv clo_tag k boundG (Vfun rho1 B1 f1)
+    (cc_approx_val clo_tag k boundG (Vfun rho1 B1 f1)
                    (Vconstr clo_tag [(Vfun rho2 B2 f2) ; env])) ->
     Fun_inv k (M.set f (Vfun rho1 B1 f1) rho)
             (M.set f (Vfun rho2 B2 f2) rho')
@@ -571,7 +571,7 @@ Section Closure_conversion_invariants.
   Lemma FV_inv_strong_Forall2 k rho rho' Scope GFuns Funs c Γ FVs vs1 vs2 :
     get_list FVs rho = Some vs1 ->
     M.get Γ rho' = Some (Vconstr c vs2) ->
-    Forall2 (cc_approx_val cenv clo_tag k boundG) vs1 vs2 ->
+    Forall2 (cc_approx_val clo_tag k boundG) vs1 vs2 ->
     FV_inv_strong k rho rho' Scope Funs GFuns c Γ FVs.
   Proof.
     intros Hget1 Hget2 Hall. do 2 eexists; split; eauto. 
@@ -630,7 +630,7 @@ Section Closure_conversion_invariants.
   Lemma GFun_inv_set k rho rho' GFuns f rho1 B1 f1 rho2 B2 f2:
     GFun_inv k rho rho' GFuns ->
     (forall c, f \in GFuns ->
-          cc_approx_val cenv clo_tag k boundG (Vfun rho1 B1 f1) (Vconstr clo_tag [(Vfun rho2 B2 f2) ; Vconstr c []])) ->
+          cc_approx_val clo_tag k boundG (Vfun rho1 B1 f1) (Vconstr clo_tag [(Vfun rho2 B2 f2) ; Vconstr c []])) ->
     GFun_inv k (M.set f (Vfun rho1 B1 f1) rho) (M.set f (Vfun rho2 B2 f2) rho') GFuns.
   Proof.
     intros Hinv Hv f'' v Hnin'' Hin Hget'.
